Major simplification of F_mu logrel.

F_mu/logrel.v
@@ -5,362 +5,134 @@ Import uPred.
 (** interp : is a unary logical relation. *)
 Section logrel.
   Context {Σ : iFunctor}.
+  Notation D := (valC -n> iProp lang Σ).
+  Implicit Types τi : D.
+  Implicit Types Δ : listC D.
+  Implicit Types interp : listC D → D.
 
-  (** Just to get nicer closed forms, we define extend_context_interp in three steps. *)
-  Program Definition extend_context_interp_fun1
-      (τi : valC -n> iProp lang Σ)
-      (f : varC -n> valC -n> iProp lang Σ) :
-      (varC -n> valC -n> iProp lang Σ) := λne x,
-    match x return valC -n> iProp lang Σ with O => τi | S x' => f x' end.
+  Program Definition ctx_lookup (x : var) : listC D -n> D := λne Δ,
+    from_option id (cconst True)%I (Δ !! x).
+  Solve Obligations with solve_proper_alt.
 
-  Program Definition extend_context_interp_fun2
-    (τi : valC -n> iProp lang Σ) :
-    (varC -n> valC -n> iProp lang Σ) -n>
-    (varC -n> valC -n> iProp lang Σ) := λne f, extend_context_interp_fun1 τi f.
-  Next Obligation. intros ???? Hfg x; destruct x; cbn; trivial. Qed.
+  Definition interp_unit : listC D -n> D := λne Δ w, (w = UnitV)%I.
 
-  Program Definition extend_context_interp :
-    (valC -n> iProp lang Σ) -n>
-    (varC -n> valC -n> iProp lang Σ) -n>
-    (varC -n> valC -n> iProp lang Σ) := λne τi, extend_context_interp_fun2 τi.
-  Next Obligation. intros n g h H Δ x y. destruct x; cbn; auto. Qed.
-
-  Program Definition extend_context_interp_apply :
-      ((varC -n> valC -n> iProp lang Σ)) -n>
-      ((varC -n> valC -n> iProp lang Σ) -n>
-       valC -n> iProp lang Σ) -n>
-      (valC -n> iProp lang Σ) -n> (valC -n> iProp lang Σ) := λne Δ f g,
-    f (extend_context_interp g Δ).
-  Solve Obligations with
-  repeat intros ?; (cbn + idtac);
-    try match goal with [H : _ ≡{_}≡ _|- _] => rewrite H end; trivial.
-  Next Obligation.
-    intros n Δ Δ' HΔ f g x.  cbn.
-    match goal with
-      |- _ _ ?F x ≡{n}≡ _ _ ?G x =>
-      assert (F ≡{n}≡ G) as HFG; [|rewrite HFG; trivial]
-    end.
-    apply cofe_mor_car_ne; trivial. intros y. cbn.
-    destruct y; trivial.
-  Qed.
-
-  Definition interp_unit : valC -n> iProp lang Σ := λne w, (w = UnitV)%I.
-
-  Program Definition interp_prod :
-      (valC -n> iProp lang Σ) -n> (valC -n> iProp lang Σ) -n>
-      valC -n> iProp lang Σ := λne τ1i τ2i w,
-    (∃ w1 w2, w = PairV w1 w2 ∧ τ1i w1 ∧ τ2i w2)%I.
+  Program Definition interp_prod
+      (interp1 interp2 : listC D -n> D) : listC D -n> D := λne Δ w,
+    (∃ w1 w2, w = PairV w1 w2 ∧ interp1 Δ w1 ∧ interp2 Δ w2)%I.
   Solve Obligations with solve_proper.
 
-  Program Definition interp_sum :
-      (valC -n> iProp lang Σ) -n> (valC -n> iProp lang Σ) -n>
-      valC -n> iProp lang Σ := λne τ1i τ2i w,
-    ((∃ w1, w = InjLV w1 ∧ τ1i w1) ∨ (∃ w2, w = InjRV w2 ∧ τ2i w2))%I.
+  Program Definition interp_sum
+      (interp1 interp2 : listC D -n> D) : listC D -n> D := λne Δ w,
+    ((∃ w1, w = InjLV w1 ∧ interp1 Δ w1) ∨ (∃ w2, w = InjRV w2 ∧ interp2 Δ w2))%I.
   Solve Obligations with solve_proper.
 
-  Program Definition interp_arrow :
-      (valC -n> iProp lang Σ) -n> (valC -n> iProp lang Σ) -n>
-      valC -n> iProp lang Σ := λne τ1i τ2i w,
-    (□ ∀ v, τ1i v → WP App (# w) (# v) {{ τ2i }})%I.
+  Program Definition interp_arrow
+      (interp1 interp2 : listC D -n> D) : listC D -n> D := λne Δ w,
+    (□ ∀ v, interp1 Δ v → WP App (# w) (# v) {{ interp2 Δ }})%I.
   Solve Obligations with solve_proper.
 
-  Program Definition interp_forall :
-      ((valC -n> iProp lang Σ) -n> (valC -n> iProp lang Σ)) -n>
-      valC -n> iProp lang Σ := λne τi w,
-    (∀ τ'i : valC -n> iProp lang Σ,
-      □ (■ (∀ v, PersistentP (τ'i v)) → WP TApp (# w) {{ τi τ'i }}))%I.
+  Program Definition interp_forall
+      (interp : listC D -n> D) : listC D -n> D := λne Δ w,
+    (□ ∀ τi : D,
+      ■ (∀ v, PersistentP (τi v)) → WP TApp (# w) {{ interp (τi :: Δ) }})%I.
   Solve Obligations with solve_proper.
 
-  Program Definition interp_rec_pre :
-      ((valC -n> iProp lang Σ) -n> (valC -n> iProp lang Σ)) -n>
-      (valC -n> iProp lang Σ) -n>
-      (valC -n> iProp lang Σ) := λne τi rec_appr w,
-    (□ (∃ v, w = FoldV v ∧ ▷ τi rec_appr v))%I.
-  Solve Obligations with solve_proper.
+  Definition interp_rec1
+      (interp : listC D -n> D) (Δ : listC D) (τi : D) : D := λne w,
+    (□ (∃ v, w = FoldV v ∧ ▷ interp (τi :: Δ) v))%I.
 
-  Global Instance interp_rec_pre_contr
-      (τi : (valC -n> iProp lang Σ) -n> (valC -n> iProp lang Σ)) :
-    Contractive (interp_rec_pre τi).
+  Global Instance interp_rec1_contractive
+    (interp : listC D -n> D) (Δ : listC D) : Contractive (interp_rec1 interp Δ).
   Proof.
-    intros n f g H w; cbn.
-    apply always_ne, exist_ne; intros e; apply and_ne; trivial.
-    apply later_contractive =>i Hi. rewrite H; trivial.
+    intros n τi1 τi2 H w; cbn.
+    apply always_ne, exist_ne; intros v; apply and_ne; trivial.
+    apply later_contractive =>i Hi. by rewrite H.
   Qed.
 
-  Program Definition interp_rec :
-    ((valC -n> iProp lang Σ) -n> (valC -n> iProp lang Σ)) -n>
-    (valC -n> iProp lang Σ) := λne τi, fixpoint (interp_rec_pre τi).
-  Next Obligation. intros n f g H; apply fixpoint_ne => z; rewrite H; trivial. Qed.
+  Program Definition interp_rec (interp : listC D -n> D) : listC D -n> D := λne Δ,
+    fixpoint (interp_rec1 interp Δ).
+  Next Obligation.
+    intros interp n Δ1 Δ2 H; apply fixpoint_ne => τi w. solve_proper.
+  Qed.
 
-  Program Fixpoint interp (τ : type) {struct τ} :
-      (varC -n> (valC -n> iProp lang Σ)) -n> valC -n> iProp lang Σ :=
-    match τ with
-    | TUnit => λne Δ, interp_unit
-    | TProd τ1 τ2 => λne Δ, interp_prod (interp τ1 Δ) (interp τ2 Δ)
-    | TSum τ1 τ2 => λne Δ, interp_sum (interp τ1 Δ) (interp τ2 Δ)
-    | TArrow τ1 τ2 => λne Δ, interp_arrow (interp τ1 Δ) (interp τ2 Δ)
-    | TVar v => λne Δ : varC -n> (valC -n> iProp lang Σ), (Δ v)
-    | TForall τ' => λne Δ, interp_forall (extend_context_interp_apply Δ (interp τ'))
-    | TRec τ' => λne Δ, interp_rec (extend_context_interp_apply Δ (interp τ'))
+  Fixpoint interp (τ : type) : listC D -n> D :=
+    match τ return _ with
+    | TUnit => interp_unit
+    | TProd τ1 τ2 => interp_prod (interp τ1) (interp τ2)
+    | TSum τ1 τ2 => interp_sum (interp τ1) (interp τ2)
+    | TArrow τ1 τ2 => interp_arrow (interp τ1) (interp τ2)
+    | TVar x => ctx_lookup x
+    | TForall τ' => interp_forall (interp τ')
+    | TRec τ' => interp_rec (interp τ')
     end%I.
-  Solve Obligations with
-  repeat intros ?; match goal with [H : _ ≡{_}≡ _|- _] => rewrite H end; trivial.
 
-  Global Instance interp_Persistent
-      τ (Δ : varC -n> valC -n> iProp lang Σ) {HΔ : ∀ x v, PersistentP (Δ x v)} :
-    ∀ v, PersistentP (interp τ Δ v).
+  Class ctx_PersistentP Δ :=
+    ctx_persistentP : Forall (λ τi, ∀ v, PersistentP (τi v)) Δ.
+  Global Instance ctx_persistent_nil : ctx_PersistentP [].
+  Proof. by constructor. Qed.
+  Global Instance ctx_persistent_cons τi Δ :
+    (∀ v, PersistentP (τi v)) → ctx_PersistentP Δ → ctx_PersistentP (τi :: Δ).
+  Proof. by constructor. Qed.
+  Global Instance ctx_persistent_lookup Δ x v :
+    ctx_PersistentP Δ → PersistentP (ctx_lookup x Δ v).
+  Proof. intros HΔ; revert x; induction HΔ=>-[|?] /=; apply _. Qed.
+
+  Global Instance interp_var_persistent τ Δ v :
+    ctx_PersistentP Δ → PersistentP (interp τ Δ v).
   Proof.
-    revert Δ HΔ.
-    induction τ; cbn; intros Δ HΔ v; try apply _.
-    rewrite /PersistentP /interp_rec fixpoint_unfold /interp_rec_pre; cbn.
-    apply always_intro'; trivial.
+    revert v Δ; induction τ=> v Δ HΔ; simpl; try apply _.
+    rewrite /PersistentP /interp_rec fixpoint_unfold /interp_rec1 /=.
+    by apply always_intro'.
   Qed.
 
-  Global Instance extend_context_interp_Persistent
-      (f : valC -n> iProp lang Σ) (Δ : varC -n> valC -n> iProp lang Σ)
-      (Hf : ∀ v, PersistentP (f v))
-      {HΔ : ∀ x v, PersistentP (Δ x v)} :
-    ∀ x v, PersistentP (@extend_context_interp f Δ x v).
-  Proof. intros x v. destruct x; cbn; trivial. Qed.
-
-  Local Ltac properness :=
-    repeat
-    match goal with
-    | |- (∃ _: _, _)%I ≡ (∃ _: _, _)%I => apply exist_proper =>?
-    | |- (∀ _: _, _)%I ≡ (∀ _: _, _)%I => apply forall_proper =>?
-    | |- (_ ∧ _)%I ≡ (_ ∧ _)%I => apply and_proper
-    | |- (_ ∨ _)%I ≡ (_ ∨ _)%I => apply or_proper
-    | |- (_ → _)%I ≡ (_ → _)%I => apply impl_proper
-    | |- (WP _ {{ _ }})%I ≡ (WP _ {{ _ }})%I => apply wp_proper =>?
-    | |- (▷ _)%I ≡ (▷ _)%I => apply later_proper
-    | |- (□ _)%I ≡ (□ _)%I => apply always_proper
-    end.
-
-  Lemma interp_unused_contex_irrel
-      (m n : nat) (Δ Δ' : varC -n> valC -n> iProp lang Σ)
-      (HΔ : ∀ v, Δ (if lt_dec v m then v else (n + v)) ≡
-                   Δ' (if lt_dec v m then v else (n + v)))
-      (τ : type) :
-    interp τ.[iter m up (ren (+n))] Δ ≡ interp τ.[iter m up (ren (+n))] Δ'.
+  Lemma interp_weaken Δ1 Π Δ2 τ :
+    interp τ.[iter (length Δ1) up (ren (+ length Π))] (Δ1 ++ Π ++ Δ2)
+    ≡ interp τ (Δ1 ++ Δ2).
   Proof.
-    revert m n Δ Δ' HΔ.
-    induction τ; intros m n Δ Δ' HΔ v; cbn; auto.
-    - properness; trivial; try apply IHτ1; try apply IHτ2; trivial.
-    - properness; trivial; try apply IHτ1; try apply IHτ2; trivial.
-    - properness; trivial; try apply IHτ1; try apply IHτ2; trivial.
-    - match goal with
-        |- _ _ ?f ?x ≡ _ _ ?g ?x =>
-        assert (f ≡ g) as Hfg; [|rewrite Hfg; trivial]
-      end.
-      apply fixpoint_proper => ??; cbn.
-      properness; trivial.
-      change (up (iter m up (ren (+n)))) with (iter (S m) up (ren (+n))).
-      apply IHτ.
-      {
-        intros x y. destruct x; cbn; trivial.
-        destruct lt_dec.
-        - specialize (HΔ x); destruct lt_dec; auto with omega.
-        - destruct (n + S x) as [|k] eqn:Heq; trivial.
-          specialize (HΔ x); destruct lt_dec; auto with omega.
-          replace (n + x) with k in HΔ by omega; trivial.
-      }
-    -  rewrite iter_up. destruct lt_dec; cbn.
-       + specialize (HΔ x); destruct lt_dec; auto with omega.
-       + asimpl; unfold ids; cbn.
-         specialize (HΔ x); destruct lt_dec; auto with omega.
-         replace (m + n + (x - m)) with (n + x) by omega. trivial.
-    - properness; trivial.
-      change (up (iter m up (ren (+n)))) with (iter (S m) up (ren (+n))).
-      apply IHτ.
-      {
-        intros x y. destruct x; cbn; trivial.
-        destruct lt_dec.
-        - specialize (HΔ x); destruct lt_dec; auto with omega.
-        - destruct (n + S x) as [|k] eqn:Heq; trivial.
-          specialize (HΔ x); destruct lt_dec; auto with omega.
-          replace (n + x) with k in HΔ by omega; trivial.
-      }
+    revert Δ1 Π Δ2. induction τ=> Δ1 Π Δ2; simpl; auto.
+    - intros w; simpl; properness; auto. by apply IHτ1. by apply IHτ2.
+    - intros w; simpl; properness; auto. by apply IHτ1. by apply IHτ2.
+    - intros w; simpl; properness; auto. by apply IHτ1. by apply IHτ2.
+    - apply fixpoint_proper=> τi w /=.
+      properness; auto. apply (IHτ (_ :: _)).
+    - rewrite iter_up; destruct lt_dec as [Hl | Hl]; simpl.
+      { by rewrite !lookup_app_l. }
+      change (uPredC (iResUR lang Σ)) with (iProp lang Σ).
+      rewrite !lookup_app_r; [|lia ..]. do 2 f_equiv. lia. done.
+    - intros w; simpl; properness; auto. apply (IHτ (_ :: _)).
   Qed.
 
-  Program Definition hop_context_interp (m n : nat) :
-      (varC -n> valC -n> iProp lang Σ) -n>
-      (varC -n> valC -n> iProp lang Σ) := λne Δ v,
-    if lt_dec v m then Δ v else Δ (v - n).
-  Next Obligation. intros ?????? Hxy; destruct Hxy; trivial. Qed.
-  Next Obligation.
-    intros ????? Hfg ?; cbn. destruct lt_dec; rewrite Hfg; trivial.
-  Qed.
-
-  Lemma extend_bofore_hop_context_interp (m n : nat)
-      (Δ : varC -n> valC -n> iProp lang Σ)
-      (τi : valC -n> iProp lang Σ) (v : var) :
-    (extend_context_interp τi (hop_context_interp m n Δ)
-                              (if lt_dec v (S m) then v else n + v))
-    ≡ (hop_context_interp (S m) n (extend_context_interp τi Δ)
-                                  (if lt_dec v (S m) then v else n + v)).
+  Lemma interp_subst_up Δ1 Δ2 τ τ' :
+    interp τ (Δ1 ++ interp τ' Δ2 :: Δ2)
+    ≡ interp τ.[iter (length Δ1) up (τ' .: ids)] (Δ1 ++ Δ2).
   Proof.
-    destruct v; cbn; trivial.
-    repeat (destruct lt_dec; cbn); auto with omega.
-    destruct (n + S v - n) eqn:Heq1;
-      destruct (n + S v) eqn:Heq2; try destruct lt_dec; auto with omega.
-    match goal with
-      [ |- _ _ _ Δ ?a ≡ _ _ _ Δ ?b] => assert (Heq : a = b) by omega; rewrite Heq; trivial
-    end.
+    revert Δ1 Δ2; induction τ=> Δ1 Δ2; simpl.
+    - done.
+    - intros w; simpl; properness; auto. by apply IHτ1. by apply IHτ2.
+    - intros w; simpl; properness; auto. by apply IHτ1. by apply IHτ2.
+    - intros w; simpl; properness; auto. by apply IHτ1. by apply IHτ2.
+    - apply fixpoint_proper=> τi w /=.
+      properness; auto. apply (IHτ (_ :: _)).
+    - rewrite iter_up; destruct lt_dec as [Hl | Hl]; simpl.
+      { by rewrite !lookup_app_l. }
+      change (uPredC (iResUR lang Σ)) with (iProp lang Σ).
+      rewrite !lookup_app_r; [|lia ..].
+      destruct (x - length Δ1) as [|n] eqn:?; simpl.
+      { symmetry. asimpl. apply (interp_weaken [] Δ1 Δ2 τ'). }
+      change (uPredC (iResUR lang Σ)) with (iProp lang Σ).
+      rewrite !lookup_app_r; [|lia ..]. do 2 f_equiv. lia. done.
+    - intros w; simpl; properness; auto. apply (IHτ (_ :: _)).
   Qed.
 
-  Lemma interp_subst_weaken
-      (m n : nat) (Δ : varC -n> valC -n> iProp lang Σ) (τ : type) :
-    interp τ Δ ≡ interp τ.[iter m up (ren (+n))] (hop_context_interp m n Δ).
-  Proof.
-    revert m n Δ.
-    induction τ; intros m n Δ v; cbn -[extend_context_interp]; auto.
-    - properness; trivial; try apply IHτ1; try apply IHτ2.
-    - properness; trivial; try apply IHτ1; try apply IHτ2.
-    - properness; trivial; try apply IHτ1; try apply IHτ2.
-    - match goal with
-        |- _ _ ?f ?x ≡ _ _ ?g ?x =>
-        assert (f ≡ g) as Hfg; [|rewrite Hfg; trivial]
-      end.
-      apply fixpoint_proper => ??; cbn -[extend_context_interp].
-      properness; trivial.
-      rewrite IHτ.
-      change (up (iter m up (ren (+n)))) with (iter (S m) up (ren (+n))).
-      apply interp_unused_contex_irrel.
-      intros w; rewrite extend_bofore_hop_context_interp; trivial.
-    - rewrite iter_up.
-      asimpl; unfold ids; cbn; destruct lt_dec; cbn; destruct lt_dec; auto with omega.
-      replace (m + n + (x - m)) with (x + n) by omega.
-      replace (x + n - n) with x; trivial.
-      { unfold var in *; omega. }
-    - properness; trivial.
-      change (up (iter m up (ren (+n)))) with (iter (S m) up (ren (+n))).
-      rewrite IHτ.
-      apply interp_unused_contex_irrel.
-      intros w; rewrite extend_bofore_hop_context_interp; trivial.
-  Qed.
+  Lemma interp_subst Δ2 τ τ' : interp τ (interp τ' Δ2 :: Δ2) ≡ interp τ.[τ'/] Δ2.
+  Proof. apply (interp_subst_up []). Qed.
 
-  Lemma interp_ren_S (τ : type)
-      (Δ : varC -n> valC -n> iProp lang Σ)
-      (τi : valC -n> iProp lang Σ) :
-    interp τ Δ ≡ interp τ.[ren (+1)] (extend_context_interp τi Δ).
-  Proof.
-    rewrite (interp_subst_weaken 0 1).
-    apply interp_unused_contex_irrel.
-    { clear. intros [|v]; cbn; trivial. }
-  Qed.
-
-  Local Opaque eq_nat_dec.
-
-  Program Definition context_interp_insert (m : nat) :
-    (valC -n> iProp lang Σ) -n>
-    (varC -n> valC -n> iProp lang Σ) -n>
-    (varC -n> valC -n> iProp lang Σ) := λne τi Δ v,
-      if lt_dec v m then Δ v else if eq_nat_dec v m then τi else Δ (v - 1).
-  Next Obligation. intros m τi Δ n x y Hxy; destruct Hxy; trivial. Qed.
-  Next Obligation.
-    intros m τi n Δ Δ' HΔ x; cbn;
-      destruct lt_dec; try destruct eq_nat_dec; auto.
-  Qed.
-  Next Obligation.
-    intros m n f g Hfg F Δ x; cbn;
-      destruct lt_dec; try destruct eq_nat_dec; auto.
-  Qed.
-
-  Lemma extend_context_interp_insert (m : nat)
-      (τi : valC -n> iProp lang Σ)
-      (Δ : varC -n> valC -n> iProp lang Σ)
-      (Ti : valC -n> iProp lang Σ) :
-    extend_context_interp Ti (context_interp_insert m τi Δ)
-    ≡ context_interp_insert (S m) τi (extend_context_interp Ti Δ).
-  Proof.
-    intros [|v]; cbn; trivial.
-    repeat destruct lt_dec; trivial;
-      repeat destruct eq_nat_dec; cbn; auto with omega.
-    destruct v; cbn; auto with omega.
-    replace (v - 0) with v by omega; trivial.
-  Qed.
-
-  Lemma context_interp_insert_O_extend
-      (τi : valC -n> iProp lang Σ) (Δ : varC -n> valC -n> iProp lang Σ) :
-    context_interp_insert O τi Δ ≡ extend_context_interp τi Δ.
-  Proof.
-    intros [|v]; cbn; trivial.
-    repeat destruct lt_dec; trivial;
-      repeat destruct eq_nat_dec; cbn; auto with omega.
-    destruct v; cbn; auto with omega.
-  Qed.
-
-  Lemma iter_up_subst_type (m : nat) (τ : type) (x : var) :
-    iter m up (τ .: ids) x =
-      if lt_dec x m then ids x else
-        if eq_nat_dec x m then τ.[ren (+m)] else ids (x - 1).
-  Proof.
-    revert x τ.
-    induction m; intros x τ; cbn.
-    - destruct x; cbn.
-      + destruct eq_nat_dec; auto with omega.
-        asimpl; trivial.
-      + destruct eq_nat_dec; auto with omega.
-    - destruct x; asimpl; trivial.
-      rewrite IHm.
-      repeat destruct lt_dec; repeat destruct eq_nat_dec;
-        asimpl; auto with omega.
-  Qed.
-
-  Lemma interp_subst_iter_up
-      (m : nat)
-      (Δ : varC -n> valC -n> iProp lang Σ)
-      (τ : type) (τ' : type) :
-    interp τ (context_interp_insert m (interp τ'.[ren (+m)] Δ) Δ)
-    ≡ interp τ.[iter m up (τ' .: ids)] Δ.
-  Proof.
-    revert m Δ.
-    induction τ; intros m Δ v; cbn -[extend_context_interp]; auto.
-    - properness; trivial; try apply IHτ1; try apply IHτ2.
-    - properness; trivial; try apply IHτ1; try apply IHτ2.
-    - properness; trivial; try apply IHτ1; try apply IHτ2.
-    - match goal with
-        |- _ _ ?f ?x ≡ _ _ ?g ?x =>
-        assert (f ≡ g) as Hfg; [|rewrite Hfg; trivial]
-      end.
-      apply fixpoint_proper => ??; cbn -[extend_context_interp].
-      properness; trivial.
-      rewrite extend_context_interp_insert.
-      change (up (iter m up (τ' .: ids))) with (iter (S m) up (τ' .: ids)).
-      rewrite -IHτ.
-      replace (τ'.[ren (+S m)]) with ((τ'.[ren (+m)]).[ren (+1)]) by (asimpl; trivial).
-      rewrite -interp_ren_S; trivial.
-    - rewrite iter_up_subst_type.
-      repeat destruct lt_dec; repeat destruct eq_nat_dec;
-        unfold ids; asimpl; trivial.
-    - properness; trivial.
-      rewrite extend_context_interp_insert.
-      change (up (iter m up (τ' .: ids))) with (iter (S m) up (τ' .: ids)).
-      rewrite -IHτ.
-      replace (τ'.[ren (+S m)]) with ((τ'.[ren (+m)]).[ren (+1)]) by (asimpl; trivial).
-      rewrite -interp_ren_S; trivial.
-  Qed.
-
-  Lemma interp_subst
-      (Δ : varC -n> valC -n> iProp lang Σ)
-      (τ : type) (τ' : type) :
-    interp τ (extend_context_interp (interp τ' Δ) Δ) ≡ interp τ.[τ'/] Δ.
-  Proof.
-    rewrite -(interp_subst_iter_up O Δ τ τ').
-    rewrite context_interp_insert_O_extend.
-    asimpl; trivial.
-  Qed.
-
-  Lemma zip_with_context_interp_subst
-        (Δ : varC -n> valC -n> iProp lang Σ) (Γ : list type)
-        (vs : list valC) (τi : valC -n> iProp lang Σ) :
+  Lemma context_interp_ren_S Δ (Γ : list type) (vs : list val) τi :
     ([∧] zip_with (λ τ, interp τ Δ) Γ vs)
-    ⊣⊢ ([∧] zip_with (λ τ, interp τ (extend_context_interp τi Δ))
-                    (map (λ t : type, t.[ren (+1)]) Γ) vs).
+    ⊣⊢ ([∧] zip_with (λ τ, interp τ.[ren (+1)] (τi :: Δ)) Γ vs).
   Proof.
-    revert Δ vs τi.
-    induction Γ as [|Γ]; intros Δ vs τi; cbn; trivial.
-    destruct vs; cbn; trivial.
-    apply and_proper. apply interp_ren_S. apply IHΓ.
+    revert Δ vs τi; induction Γ=> Δ [|v vs] τi; simpl; auto.
+    apply and_proper; auto.
+    symmetry. apply (interp_weaken [] [τi] Δ).
   Qed.
 End logrel.
