F_mu/soundness.v
@@ -2,34 +2,22 @@ From iris_logrel.F_mu Require Export fundamental.
 From iris.proofmode Require Import tactics.
 From iris.program_logic Require Import adequacy.
 
-Section Soundness.
+Section soundness.
   Let Σ := #[].
 
-  Lemma empty_env_subst e : e.[env_subst []] = e.
-  Proof. change (env_subst []) with (@ids expr _). by asimpl. Qed.
-
-  Definition free_type_context : varC -n> valC -n> iProp lang (globalF Σ) :=
-    λne x y, True%I.
-
   Lemma wp_soundness e τ :
-    [] ⊢ₜ e : τ → True ⊢ WP e {{ @interp (globalF Σ) τ free_type_context }}.
+    [] ⊢ₜ e : τ → True ⊢ WP e {{ @interp (globalF Σ) τ [] }}.
   Proof.
     iIntros {H} "". rewrite -(empty_env_subst e).
     by iApply (@typed_interp _ _ _ []).
   Qed.
 
-  Theorem Soundness e τ :
-    [] ⊢ₜ e : τ →
-    ∀ e' thp, rtc step ([e], tt) (e' :: thp, tt) →
-              ¬ reducible e' tt → is_Some (to_val e').
+  Theorem soundness e τ e' thp :
+    [] ⊢ₜ e : τ → rtc step ([e], ()) (e' :: thp, ()) →
+    is_Some (to_val e') ∨ reducible e' ().
   Proof.
-    intros H1 e' thp Hstp Hnr.
-    eapply wp_soundness in H1; eauto.
-    edestruct (@wp_adequacy_reducible lang (globalF Σ) ⊤
-                                     (interp τ free_type_context)
-                                     e e' (e' :: thp) tt ∅) as [Ha|Ha];
-      eauto using ucmra_unit_valid; try tauto.
-    - iIntros "H". iApply H1.
+    intros ??. eapply wp_adequacy_reducible; eauto using ucmra_unit_valid.
+    - iIntros "H". by iApply wp_soundness.
     - constructor.
   Qed.
-End Soundness.
+End soundness.
